More overapproximation, new tests

hol/p4_testLib.sig
@@ -2,6 +2,7 @@ signature p4_testLib =
 sig
   include Abbrev
 
+val fixedwidth_freevars_fromindex_ty : string * int * int * hol_type -> term
 val fixedwidth_freevars_fromindex : string * int * int -> term
 val fixedwidth_freevars : string * int -> term
 
